Execution time

6502_LightEventB/AbstractRegister6502.v
@@ -1,34 +1,87 @@
+Require Import MachineInt.
+
 Module AbstractRegister6502.
 
 Module Context.
 
-Parameter reg: Type.
+Parameter reg: byte.
 
 End Context.
 
-Record Registers : Set := mkState {
+Inductive Reg8 : Set := A : Reg8 | X : Reg8 | Y : Reg8 | STATUS : Reg8 | FLAGS : Reg8.
 
+Record RegF : Set := mkState {
+    RA: byte;
+    RX: byte;
+    RY: byte;
+    RSTATUS: byte;
+    RFLAGS: byte }.
 
-
-
-}.
-
-Record State : Set = mkState {
-
-
-}.
-
-Definition Inv_1 (B: State) : Prop := True.
+Definition Inv_1 (B: RegF) : Prop := True.
 
 Module Init.
 
 Definition Guard : Prop := True.
-Definition action : State := mkState .
+Definition action : RegF := mkState (Byte.repr 0) (Byte.repr 0) (Byte.repr 0) (Byte.repr 0) (Byte.repr 0).
 
-Theorem PO_Safety: forall S: State,
-Guard S -> let S' := action S in Inv_1 S.
-
+Lemma PO_Safety: forall S: RegF, Guard -> let S' := action in Inv_1 S.
+intros S.
+simpl.
+compute.
+intro.
+exact H.
+Qed.
 
 End Init.
+
+Module EventSetRegister.
+
+Definition setReg8 : RegF -> Reg8 -> byte -> RegF :=
+  fun RF r b =>
+    match r with
+        A => mkState (b) (RF.(RX)) (RF.(RY)) (RF.(RSTATUS)) (RF.(RFLAGS))
+      | X => mkState (RF.(RA)) (b) (RF.(RY)) (RF.(RSTATUS)) (RF.(RFLAGS))
+      | Y => mkState (RF.(RA)) (RF.(RX)) (b) (RF.(RSTATUS)) (RF.(RFLAGS))
+      | STATUS => mkState (RF.(RA)) (RF.(RX)) (RF.(RY)) (b) (RF.(RFLAGS))
+      | FLAGS => mkState (RF.(RA)) (RF.(RX)) (RF.(RY)) (RF.(RSTATUS)) (b)
+    end.
+
+Definition Guard : Prop := True.
+Definition action (S : RegF) (r : Reg8) (b : byte) : RegF := setReg8 S r b.
+
+Lemma PO_Safety: forall S: RegF, Guard -> let S' := action in Inv_1 S.
+intros S.
+simpl.
+compute.
+intro.
+exact H.
+Qed.
+
+End EventSetRegister.
+
+Module EventGetRegisterValue.
+
+Definition getReg8 : RegF -> Reg8 -> byte :=
+  fun RF r =>
+    match r with
+        A => RF.(RA)
+      | X => RF.(RX)
+      | Y => RF.(RY)
+      | STATUS => RF.(RSTATUS)
+      | FLAGS => RF.(RFLAGS)
+    end.
+
+Definition Guard : Prop := True.
+Definition action (S : RegF) (r : Reg8) : byte := getReg8 S r.
+
+Lemma PO_Safety: forall S: RegF, Guard -> let S' := action in Inv_1 S.
+intros S.
+simpl.
+compute.
+intro.
+exact H.
+Qed.
+
+End EventGetRegisterValue.
 
 End AbstractRegister6502.
