6502_LightEventB/ConcreteRegister6502.v
@@ -2,36 +2,5 @@ Require Import AbstractRegister6502.
 
 Module ConcreteRegister6502.
 
-Module Context.
-
-End Context.
-
-Record Registers : Set := mkState {
-
-
-
-
-}.
-
-Record State : Set = mkState {
-
-
-}.
-
-Definition Inv_1 (B: State) : Prop := True.
-Definition Glue_1 : Prop := True.
-
-
-Module Init.
-
-Definition Guard : Prop := True.
-Definition action : State := mkState.
-
-
-Theorem PO_Safety: forall S: State,
-Guard S -> let S' := action S in Inv_1 S.
-
-
-End Init.
 
 End ConcreteRegister6502.
