M6502_Prog.v
@@ -1,27 +1,85 @@
-Definition StartIP : Z := 0.
+Require Import MachineInt.
+Require Import M6502_Reg.
+Require Import M6502_Instr.
+Require Import M6502_Mem.
+Require Import M6502_Proc.
+Require Import Coqlib.
+Require Import ZArith.
+Require Import List.
+Open Scope Z_scope.
 
-Definition R8 : RegFile8 :=
-  fun (r : Reg8) =>
-    match r with
-      | A => Byte.repr 0
-      | X => Byte.repr 0
-      | Y => Byte.repr 0
-      | FLAGS => Byte.repr 0
-      | STATUS => Byte.repr 0
+Section Repeat.
+
+  Variable A : byte.
+  Fixpoint repeat (x : byte) (n: nat ) :=
+    match n with
+      | O => nil
+      | S k => x::(repeat x k)
     end.
 
-Definition R16 :RegFile16 :=
-  fun (r : Reg16) =>
-    match r with
-      | PC => Word.repr StartPC
-    end.
+  Theorem repeat_length x n:
+    length (repeat x n) = n.
+  Proof.
+    induction n as [| k Hrec]; simpl; rewrite ?Hrec; reflexivity.
+  Qed.
 
-Definition StartR : RegFile := (R8, R16).
+  Theorem repeat_spec n x y:
+    In y (repeat x n) -> y=x.
+  Proof.
+    induction n as [|k Hrec]; simpl; destruct 1; auto.
+  Qed.
 
-Definition StartP : Program := (StartM, StartR).
+End Repeat.
+
+Definition StartR : RegF := mkState (Byte.repr 0) (Byte.repr 0) (Byte.repr 0) (Byte.repr 0) (Byte.repr 0) (Word.repr 0).
+
+Definition StartM : Mem := singleList 0 (repeat (Byte.repr 0) 64).
+
+Definition StartP : State := (StartR, StartM).
 
 Definition prog1 : list Instr :=
   (LDA_ir (Byte.repr 1)) ::
   (LDX_ir (Byte.repr 2)) ::
   (LDY_ir (Byte.repr 0)) ::
   nil.
+
+Fixpoint find_instr (pos: Z) (code: list Instr) : option Instr :=
+  match code with
+  | nil => None
+  | i :: il => if zeq pos 0 then Some i else find_instr (pos - 1) il
+  end.
+
+Fixpoint step (S1 : State) (p: list Instr) : option State :=
+      match find_instr (Word.intval (_pc S1)) p with
+        Some i => match exec_instr i S1 with
+                    Next S2 => Some S2
+                    |Stuck => None
+                    end
+        | None => None
+        end.
+
+Eval compute in step StartP prog1.
+
+Inductive ste: Label -> list Instr -> State -> State -> Prop :=
+  | exec_step_O: forall S1, forall p, ste 0 p S1 S1
+  | exec_step_n:
+      forall cpc p i S1 S2,
+      Word.intval (_pc S1) = cpc ->
+      find_instr (cpc) p = Some i ->
+      exec_instr i S1 = Next S2 ->
+      ste (Word.intval (_pc S2)) p S1 S2.
+
+Eval apply in ste 0 prog1 StartP StartP.
+
+Fixpoint run (S1 : State) (p: list Instr) (n : nat) : State :=
+  match n with
+  | 0%nat => S1
+  | S n' => match step S1 p with
+              | Some S2 => run S2 p n'
+              | None => S1
+              end
+end.
+
+(*Eval compute in run StartP prog1.*)
+
+(*Definition Safe (S:State) : Prop := forall n, exists S', step n S S'.*)
